tmp

theories/datatypes_properties.v
@@ -10,17 +10,6 @@ Unset Strict Implicit.
 Unset Printing Implicit Defensive.
 
 
-(*
-Canonical Structure funcaddr_eqType :=
-  Eval hnf in EqType funcaddr nat_eqMixin.
-Canonical Structure tableaddr_eqType :=
-  Eval hnf in EqType tableaddr nat_eqMixin.
-Canonical Structure memaddr_eqType :=
-  Eval hnf in EqType memaddr nat_eqMixin.
-Canonical Structure globaladdr_eqType :=
-  Eval hnf in EqType globaladdr nat_eqMixin.
-*)
-
 Definition ascii_eq_dec : forall tf1 tf2 : Ascii.ascii,
   {tf1 = tf2} + {tf1 <> tf2}.
 Proof. decidable_equality. Defined.
@@ -204,16 +193,6 @@ Definition eqvalue_refP : Equality.axiom value_ref_eqb :=
 
 Canonical Structure value_ref_eqMixin := EqMixin eqvalue_refP.
 Canonical Structure value_ref_eqType := Eval hnf in EqType value_ref value_ref_eqMixin.
-(*
-(* TODO: update *)
-(** Some helper functions for [value] that can safely extract. **)
-Definition value_rec_safe (P : Type)
-           (i32 : Wasm_int.Int32.int -> P)
-           (i64 : Wasm_int.Int64.int -> P)
-           (f32 : Wasm_float.FloatSize32.T -> P)
-           (f64 : Wasm_float.FloatSize64.T -> P) v : P :=
-  value_rect i32 i64 f32 f64 v.
-*)
 
 (** Induction scheme for [basic_instruction]. **)
 Definition basic_instruction_rect' :=
@@ -246,7 +225,113 @@ Definition eqinstanceP : Equality.axiom instance_eqb :=
 Canonical Structure instance_eqMixin := EqMixin eqinstanceP.
 Canonical Structure instance_eqType := Eval hnf in EqType instance instance_eqMixin.
 
+(** Decidable equality of lholed without pulling in unnecessary 
+    equality axioms **)
+Section lholed_eqdec.
 
+Definition lholed_cast {k k'} (lh: lholed k) (Heq: k = k'): lholed k' :=
+  eq_rect k lholed lh k' Heq.
+
+(* Some combinations of theorem from standard library should give these as well,
+   but it's not clear which ones are axiom free *)
+Theorem nat_eqdec_refl: forall k, Nat.eq_dec k k = left (erefl k).
+Proof.
+  elim => //=.
+  move => k IH.
+  by rewrite IH.
+Defined.
+
+Definition nat_eqdec_canon k k' (H: k = k') : k = k' :=
+  match (Nat.eq_dec k k') with
+  | left e => e
+  | right ne => False_ind _ (ne H)
+  end.
+
+Theorem nat_eqdec_aux: forall (k: nat) (H: k = k), H = nat_eqdec_canon H.
+Proof.
+  move => k H.
+  case H.
+  unfold nat_eqdec_canon.
+  by rewrite nat_eqdec_refl.
+Defined.
+
+Theorem nat_eqdec_unique: forall (k: nat) (H: k = k), H = erefl k.
+Proof.
+  move => k H.
+  rewrite (nat_eqdec_aux H).
+  unfold nat_eqdec_canon.
+  by rewrite nat_eqdec_refl.
+Defined.
+
+Theorem lh_cast_eq {k} (lh: lholed k) (Heq: k = k):
+  @lholed_cast k k lh Heq = lh.
+Proof.
+  by rewrite (nat_eqdec_unique Heq).
+Qed.
+
+Ltac decide_eq_arg x y :=
+  let Heq := fresh "Heq" in
+  let Hcontra := fresh "Hcontra" in
+  destruct (x == y) eqn:Heq; move/eqP in Heq; subst; last by right; move => Hcontra; injection Hcontra.
+
+(* Destruct principle for a (lh n).
+   Usage: either direct application, or `destruct ... using lh_case.` *)
+Definition lh_case: forall n (P: lholed n -> Type),
+    (forall (H: 0 = n) vs es, P (lholed_cast (LH_base vs es) H)) ->
+    (forall n' (H: S n' = n) vs k es (lh: lholed n') es', P (lholed_cast (LH_rec vs k es lh es') H)) ->
+    (forall (lh: lholed n), P lh).
+Proof.
+  move => n P H0 Hrec lh.
+  destruct lh as [lvs les | n lvs k les lh les'].
+  - by specialize (H0 (erefl 0) lvs les).
+  - by specialize (Hrec _ (erefl (S n)) lvs k les lh les'). 
+Defined.
+
+(* Decidable equality of lholed without eq_rect_eq *)
+Definition lholed_eq_dec : forall k (lh1 lh2 : lholed k), {lh1 = lh2} + {lh1 <> lh2}.
+Proof.
+  elim.
+  {
+    move => lh1.
+    eapply lh_case; last done.
+    move => H vs es; rewrite lh_cast_eq.
+    move: lh1.
+    eapply lh_case; last done.
+    move => H' vs' es'; rewrite lh_cast_eq.
+    decide_eq_arg vs' vs.
+    decide_eq_arg es' es.
+    by left.
+  }
+  {
+    move => n IH lh.
+    eapply lh_case; first done.
+    move => n1 H1 vs1 k1 es1 lh1 es1'; injection H1 as ->; rewrite lh_cast_eq.
+    move: lh.
+    eapply lh_case; first done.
+    move => n2 H2 vs2 k2 es2 lh2 es2'; injection H2 as ->; rewrite lh_cast_eq.
+    decide_eq_arg vs2 vs1.
+    decide_eq_arg k2 k1.
+    decide_eq_arg es2 es1.
+    decide_eq_arg es2' es1'.
+    destruct (IH lh1 lh2) as [ | Hneq]; subst; first by left.
+    right. move => Hcontra; apply Hneq.
+    clear - Hcontra.
+    inversion Hcontra.
+    (* This one is axiom free *)
+    apply Eqdep_dec.inj_pair2_eq_dec in H0 => //.
+    decide equality.
+  }
+Defined.
+
+Definition lholed_eqb {k} (v1 v2: lholed k) : bool := lholed_eq_dec v1 v2.
+
+Definition eqlholedP {k} :=
+  eq_dec_Equality_axiom (@lholed_eq_dec k).
+
+Canonical Structure lholed_eqMixin {k} := EqMixin (@eqlholedP k).
+Canonical Structure lholed_eqType {k} := Eval hnf in EqType (@lholed k) (@lholed_eqMixin k).
+
+End lholed_eqdec.
 
 Section Host.
 
